prove the Opapp case of exp_to_Cexp_correct
this is a good sign that the theorem statement is now correct; should
check the Letrec case also.

compiler/proofs/toIntLangProofScript.sml
@@ -1,4 +1,4 @@
-open HolKernel bossLib boolLib boolSimps lcsymtacs listTheory pairTheory pred_setTheory
+open HolKernel bossLib boolLib boolSimps lcsymtacs listTheory pairTheory pred_setTheory arithmeticTheory
 open miscLib miscTheory intLang4Theory intLangTheory toIntLangTheory compilerTerminationTheory intLangExtraTheory
 open toIntLang4ProofTheory
 val _ = new_theory "toIntLangProof"
@@ -85,7 +85,16 @@ val free_vars_i4_def = tDefine"free_vars_i4"`
   | INR (INR (_,es)) => exp_i41_size es)`)
 val _ = export_rewrites["free_vars_i4_def"]
 
-(*
+val free_vars_defs_i4_MAP = store_thm("free_vars_defs_i4_MAP",
+  ``set (free_vars_defs_i4 n es) = set (lshift (n+1) (free_vars_list_i4 es))``,
+  Induct_on`es`>>simp[] >> fs[EXTENSION] >>
+  rw[EQ_IMP_THM] >> simp[] >> metis_tac[])
+
+val free_vars_list_i4_MAP = store_thm("free_vars_list_i4_MAP",
+  ``∀es. set (free_vars_list_i4 es) = set (FLAT (MAP free_vars_i4 es))``,
+  Induct >> simp[])
+val _ = export_rewrites["free_vars_defs_i4_MAP","free_vars_list_i4_MAP"]
+
 val free_vars_exp_to_Cexp = store_thm("free_vars_exp_to_Cexp",
   ``(∀e. set (free_vars (exp_to_Cexp e)) = set (free_vars_i4 e)) ∧
     (∀es. set (free_vars_list (exps_to_Cexps es)) = set (free_vars_list_i4 es))``,
@@ -106,11 +115,73 @@ val free_vars_exp_to_Cexp = store_thm("free_vars_exp_to_Cexp",
     fs[EXTENSION] >> rw[EQ_IMP_THM] >> rw[] >> fsrw_tac[ARITH_ss][] >>
     spose_not_then strip_assume_tac >>
     first_x_assum(qspec_then`x+1`mp_tac) >> simp[] ) >>
+  rpt gen_tac >> strip_tac >>
+  fs[EXTENSION,free_vars_defs_MAP,free_vars_list_MAP] >>
+  simp[MAP_MAP_o,combinTheory.o_DEF] >>
+  fs[MEM_FLAT,MEM_MAP,PULL_EXISTS] >>
+  rw[EQ_IMP_THM] >> rw[] >> fsrw_tac[ARITH_ss][] >>
+  metis_tac[])
+val _ = export_rewrites["free_vars_exp_to_Cexp"]
+
+val no_labs_exp_to_Cexp = store_thm("no_labs_exp_to_Cexp",
+  ``(∀e. no_labs (exp_to_Cexp e)) ∧
+    (∀es. no_labs_list (exps_to_Cexps es))``,
+  ho_match_mp_tac exp_to_Cexp_ind >>
+  rw[exp_to_Cexp_def,exps_to_Cexps_MAP] >>
+  rw[EVERY_MAP,rich_listTheory.EVERY_REVERSE] >>
+  TRY (unabbrev_all_tac >>
+       fsrw_tac[DNF_ss][EVERY_MEM,MEM_MAP,FORALL_PROD] >>
+       simp[UNCURRY] >> NO_TAC) >>
+  BasicProvers.CASE_TAC >> rw[])
+val _ = export_rewrites["no_labs_exp_to_Cexp"]
+
+val (closed_i4_rules,closed_i4_ind,closed_i4_cases) = Hol_reln`
+(closed_i4 (Litv_i4 l)) ∧
+(EVERY (closed_i4) vs ⇒ closed_i4 (Conv_i4 cn vs)) ∧
+(EVERY (closed_i4) env ∧ set (free_vars_i4 b) ⊆ count (LENGTH env + 1)
+⇒ closed_i4 (Closure_i4 env b)) ∧
+(EVERY (closed_i4) env ∧ d < LENGTH defs ∧
+ EVERY (λe. set (free_vars_i4 e) ⊆ count (LENGTH env + LENGTH defs + 1)) defs
+⇒ closed_i4 (Recclosure_i4 env defs d)) ∧
+(closed_i4 (Loc_i4 n))`;
+
+val closed_i4_lit_loc_conv = store_thm("closed_i4_lit_loc_conv",
+  ``closed_i4 (Litv_i4 l) ∧ closed_i4 (Loc_i4 n) ∧
+    (closed_i4 (Conv_i4 a bs) ⇔ EVERY closed_i4 bs)``,
+  rw[closed_i4_cases])
+val _ = export_rewrites["closed_i4_lit_loc_conv"]
+
+val v_to_Cv_closed = store_thm("v_to_Cv_closed",
+  ``(∀v. closed_i4 v ⇒ Cclosed (v_to_Cv v)) ∧
+    (∀vs. EVERY closed_i4 vs ⇒ EVERY Cclosed (vs_to_Cvs vs))``,
+  ho_match_mp_tac(TypeBase.induction_of``:v_i4``) >>
+  simp[] >> rw[] >-
+    simp[Once Cclosed_cases] >>
+  pop_assum mp_tac >>
+  simp[Once closed_i4_cases] >>
+  simp[Once Cclosed_cases] >- (
+    simp[SUBSET_DEF,PULL_EXISTS] >>
+    rw[] >> rw[] >> simp[] >> res_tac >> simp[] ) >>
+  rw[MEM_MAP] >> rw[] >>
+  fs[EVERY_MEM] >> res_tac >>
+  fsrw_tac[ARITH_ss][])
+
+val csg_closed_i4_def = Define`
+  csg_closed_i4 csg ⇔
+    EVERY closed_i4 (SND(FST csg)) ∧
+    EVERY (OPTION_EVERY closed_i4) (SND csg)`
+
+val no_vlabs_v_to_Cv = store_thm("no_vlabs_v_to_Cv",
+  ``(∀v. no_vlabs (v_to_Cv v)) ∧
+    (∀vs. no_vlabs_list (vs_to_Cvs vs))``,
+  ho_match_mp_tac(TypeBase.induction_of(``:v_i4``)) >> simp[EVERY_MAP])
+val _ = export_rewrites["no_vlabs_v_to_Cv"]
 
 val exp_to_Cexp_correct = store_thm("exp_to_Cexp_correct",
   ``(∀ck env s e res. evaluate_i4 ck env s e res ⇒
        ck ∧
        set (free_vars_i4 e) ⊆ count (LENGTH env) ∧
+       EVERY closed_i4 env ∧ csg_closed_i4 s ∧
        SND res ≠ Rerr Rtype_error ⇒
        ∃Cres.
        Cevaluate (map_count_store_genv v_to_Cv s) (vs_to_Cvs env) (exp_to_Cexp e) Cres ∧
@@ -119,12 +190,13 @@ val exp_to_Cexp_correct = store_thm("exp_to_Cexp_correct",
     (∀ck env s es res. evaluate_list_i4 ck env s es res ⇒
        ck ∧
        set (free_vars_list_i4 es) ⊆ count (LENGTH env) ∧
+       EVERY closed_i4 env ∧ csg_closed_i4 s ∧
        SND res ≠ Rerr Rtype_error ⇒
        ∃Cres.
        Cevaluate_list (map_count_store_genv v_to_Cv s) (vs_to_Cvs env) (exps_to_Cexps es) Cres ∧
        csg_i4 syneq (map_count_store_genv v_to_Cv (FST res)) (FST Cres) ∧
        result_rel (LIST_REL syneq) syneq (map_result vs_to_Cvs v_to_Cv (SND res)) (SND Cres))``,
-  ho_match_mp_tac evaluate_i4_ind >>
+  ho_match_mp_tac evaluate_i4_strongind >>
   strip_tac >- rw[Once Cevaluate_cases] >>
   strip_tac >- (
     rpt gen_tac >> strip_tac >>
@@ -150,6 +222,13 @@ val exp_to_Cexp_correct = store_thm("exp_to_Cexp_correct",
     srw_tac[DNF_ss][] >> disj2_tac >> disj1_tac >>
     first_assum (split_pair_match o concl) >> fs[] >>
     first_assum (match_exists_tac o concl) >> simp[] >>
+    qpat_assum`p ⇒ q`mp_tac >>
+    discharge_hyps >- (
+      conj_tac >- (
+        fsrw_tac[ARITH_ss][SUBSET_DEF,ADD1,PULL_EXISTS] >>
+        Cases >> simp[] ) >>
+      cheat (* evaluate_i4_closed *) ) >>
+    strip_tac >>
     first_assum (mp_tac o MATCH_MP (CONJUNCT1 Cevaluate_syneq)) >>
     disch_then (exists_suff_gen_then mp_tac) >>
     disch_then (qspec_then`$=`mp_tac o CONV_RULE(SWAP_FORALL_CONV)) >>
@@ -191,10 +270,10 @@ val exp_to_Cexp_correct = store_thm("exp_to_Cexp_correct",
     simp[] >>
     rpt gen_tac >> rpt strip_tac >>
     simp[Once Cevaluate_cases] >>
-    srw_tac[DNF_ss][] >>
+    srw_tac[DNF_ss][] >> fs[] >>
     first_assum (split_pair_match o concl) >> fs[] >>
     first_assum (match_exists_tac o concl) >> simp[] >>
-    cheat ) >>
+    cheat (* CevalPrim1_correct *)) >>
   strip_tac >- simp[] >>
   strip_tac >- (
     simp[] >>
@@ -206,7 +285,99 @@ val exp_to_Cexp_correct = store_thm("exp_to_Cexp_correct",
     first_assum (match_exists_tac o concl) >> simp[] ) >>
   strip_tac >- (
     rw[] >> fs[] >>
-    cheat ) >>
+    `csg_closed_i4 s' ∧ closed_i4 v1` by (
+      cheat (* evaluate_i4_closed *) ) >>
+    `csg_closed_i4 ((count',s3),genv3) ∧ closed_i4 v2` by (
+      cheat (* evaluate_i4_closed *) ) >> fs[] >>
+    Cases_on`op = Opapp` >- (
+      simp[] >>
+      simp[Once Cevaluate_cases] >>
+      srw_tac[DNF_ss][] >>
+      disj1_tac >>
+      first_assum(split_pair_match o concl) >> fs[] >>
+      qpat_assum`syneq (v_to_Cv v1) X`mp_tac >>
+      Cases_on`v1`>>fs[do_app_i4_def] >>
+      simp[Once syneq_cases] >> rw[] >>
+      first_assum(match_exists_tac o concl) >> simp[] >>
+      simp[Once Cevaluate_cases] >>
+      simp[Once (CONJUNCT2 Cevaluate_cases),PULL_EXISTS] >>
+      first_assum(mp_tac o MATCH_MP (CONJUNCT1 Cevaluate_syneq)) >>
+      disch_then(exists_suff_gen_then mp_tac) >>
+      disch_then(qspec_then`$=`(exists_suff_then mp_tac)) >>
+      simp[syneq_exp_refl] >> strip_tac >>
+      first_assum(split_pair_match o concl) >> fs[] >>
+      first_assum(match_exists_tac o concl) >> simp[] >>
+      fs[bigStepTheory.dec_count_def] >>
+      qpat_assum`p ⇒ q`mp_tac >>
+      (discharge_hyps >- (
+        qpat_assum`closed_i4 (X Y)`mp_tac >>
+        simp[Once closed_i4_cases,ADD1] >>
+        fs[csg_closed_i4_def] >>
+        simp[EVERY_MEM,build_rec_env_i4_def,MEM_GENLIST,PULL_EXISTS] >>
+        simp[MEM_EL,PULL_EXISTS,SUBSET_DEF,AC ADD_ASSOC ADD_SYM] >>
+        strip_tac >> simp[Once closed_i4_cases] >>
+        simp[EVERY_MEM,MEM_EL,PULL_EXISTS,SUBSET_DEF,AC ADD_ASSOC ADD_SYM])) >>
+      strip_tac >>
+      imp_res_tac csg_i4_count >> fs[] >>
+      simp[Once map_count_store_genv_def] >>
+      simp[Once map_count_store_genv_def] >>
+      last_x_assum (mp_tac o MATCH_MP (CONJUNCT1 Cevaluate_no_vlabs)) >>
+      (discharge_hyps >- (
+        simp[EVERY_MAP,no_vlabs_csg_def,map_count_store_genv_def,EVERY_FILTER] >>
+        simp[EVERY_MEM] >> Cases >> simp[] )) >>
+      simp[Ntimes EVERY_MEM 2, Ntimes MEM_EL 2, PULL_EXISTS] >> strip_tac >>
+      first_x_assum(qspec_then`d2`mp_tac) >>
+      ntac 3 BasicProvers.CASE_TAC >> simp[] >> strip_tac >>
+      rator_assum`syneq_defs`mp_tac >>
+      simp_tac(srw_ss())[Once syneq_exp_cases] >>
+      disch_then(fn th => first_assum(mp_tac o MATCH_MP th)) >> simp[] >>
+      simp[syneq_cb_aux_def,EL_MAP] >> strip_tac >>
+      BasicProvers.VAR_EQ_TAC >>
+      rator_x_assum`syneq_exp`mp_tac >|[
+        qmatch_abbrev_tac`syneq_exp z1 z2 U (shift 1 1 e3) e4 ⇒ Z` >>
+        spec_shift_then_mp_tac >>
+        disch_then(qspecl_then[`z1-1`,`z1`,`λx y. if x = 0 then y = 0 else y = x+1`]mp_tac) >>
+        discharge_hyps >- (
+          simp[Abbr`z1`,Abbr`e3`] >>
+          qpat_assum`closed_i4 (Closure_i4 X Y)`mp_tac >>
+          simp[Once closed_i4_cases] ) >>
+        disch_then(mp_tac o (MATCH_MP (CONJUNCT1 syneq_exp_trans))) >>
+        disch_then(qspecl_then[`z2`,`U`,`e4`]mp_tac) >>
+        disch_then(fn th => disch_then(mp_tac o MATCH_MP th)) >>
+        map_every qunabbrev_tac[`z1`,`z2`,`U`,`e3`,`e4`,`Z`],
+        ALL_TAC] >>
+      simp[] >> strip_tac >>
+      first_x_assum(mp_tac o MATCH_MP (CONJUNCT1 Cevaluate_syneq)) >>
+      disch_then(exists_suff_gen_then mp_tac) >>
+      simp[ADD1,Once (GSYM AND_IMP_INTRO),build_rec_env_i4_def] >>
+      disch_then(fn th => first_x_assum (mp_tac o MATCH_MP th)) >>
+      disch_then(exists_suff_then mp_tac) >|[
+        discharge_hyps >- (
+          reverse conj_tac >- (
+            fs[map_count_store_genv_def] >>
+            qmatch_assum_rename_tac`csg_i4 syneq (X,MAP f genv3) (FST Y)`["X","f"] >>
+            PairCases_on`Y`>>fs[csg_i4_def] >>
+            metis_tac[EVERY2_syneq_trans,EVERY2_OPTREL_syneq_trans] ) >>
+          simp[relationTheory.O_DEF,PULL_EXISTS,syneq_cb_V_def] >>
+          Cases >> Cases >> simp[ADD1] >- metis_tac[syneq_trans] >>
+          rw[] >>
+          simp[rich_listTheory.EL_APPEND2] )
+        ,
+        discharge_hyps >- (
+          reverse conj_tac >- (
+            fs[map_count_store_genv_def] >>
+            qmatch_assum_rename_tac`csg_i4 syneq (X,MAP f genv3) (FST Y)`["X","f"] >>
+            PairCases_on`Y`>>fs[csg_i4_def] >>
+            metis_tac[EVERY2_syneq_trans,EVERY2_OPTREL_syneq_trans] ) >>
+          simp[PULL_EXISTS,syneq_cb_V_def] >>
+          Cases >> Cases >> simp[ADD1] >- metis_tac[syneq_trans] >>
+          rw[] >> simp[rich_listTheory.EL_APPEND1,rich_listTheory.EL_APPEND2] >>
+          simp[EL_MAP] >>
+          simp[Once syneq_cases] >>
+          metis_tac[])
+        ] >>
+      metis_tac[result_rel_syneq_syneq_trans,csg_i4_syneq_trans]) >>
+    cheat) >>
   strip_tac >- (
     simp[] >> rw[] >>
     rw[Once Cevaluate_cases] >>
@@ -220,6 +391,10 @@ val exp_to_Cexp_correct = store_thm("exp_to_Cexp_correct",
     qpat_assum`syneq (CRecClos X Y Z) A`mp_tac >>
     simp[Once syneq_cases] >> rw[] >>
     first_assum(match_exists_tac o concl) >> simp[] >>
+    qpat_assum`p ⇒ q`mp_tac >>
+    (discharge_hyps >- (
+       cheat (* evaluate_i4_closed *))) >>
+    strip_tac >>
     first_x_assum(mp_tac o MATCH_MP (CONJUNCT1 Cevaluate_syneq)) >>
     disch_then(exists_suff_gen_then mp_tac) >>
     disch_then(qspec_then`$=`(exists_suff_then mp_tac)) >>
@@ -233,6 +408,7 @@ val exp_to_Cexp_correct = store_thm("exp_to_Cexp_correct",
   strip_tac >- (
     simp[] >>
     rpt gen_tac >> rpt strip_tac >> fs[] >>
+    `csg_closed_i4 s'` by (cheat (* evaluate_i4_closed *)) >>
     Cases_on`op`>>fs[LET_THM] >- (
       BasicProvers.CASE_TAC >- (
         simp[Once Cevaluate_cases] >>
@@ -257,10 +433,19 @@ val exp_to_Cexp_correct = store_thm("exp_to_Cexp_correct",
       srw_tac[DNF_ss][] >>
       disj2_tac >>
       spec_shift_then_mp_tac >>
-
-      Cevaluate_syneq
-      mkshift_thm
-      need syneq theorem about shift
-*)
+      disch_then(qspecl_then[`LENGTH env`,`LENGTH env + 1`,`λx y. y = x+1`]mp_tac) >>
+      simp[] >> strip_tac >>
+      first_x_assum(mp_tac o MATCH_MP (CONJUNCT1 Cevaluate_syneq)) >>
+      disch_then(exists_suff_gen_then mp_tac) >>
+      simp[Once(GSYM AND_IMP_INTRO),ADD1] >>
+      disch_then(fn th => first_x_assum(mp_tac o MATCH_MP th)) >>
+      disch_then(exists_suff_then mp_tac) >>
+      discharge_hyps >- (
+        simp[rich_listTheory.EL_CONS,PRE_SUB1] ) >>
+      simp[EXISTS_PROD] >> strip_tac >> fs[] >>
+      first_assum(match_exists_tac o concl) >>
+      metis_tac[csg_i4_syneq_trans,exc_rel_syneq_trans] )
+    >> cheat) >>
+  cheat)
 
 val _ = export_theory()
